SafeVerifyTest/BvDecide/Test.lean
@@ -1,0 +1,4 @@
+import Std.Tactic.BVDecide
+
+def target_thm (x : BitVec 32) : x + 0 = x := by
+  bv_decide
